language_formal/spark2014_semantics/checks.v
@@ -1,0 +1,508 @@
+Require Import language.
+Require Import values.
+Require Import util.
+
+(** * Run Time Check Rules *)
+(** ** check rules marking what and where to check *)
+(**
+      - Do_Division_Check
+       
+       This flag is set on a division operator (/ mod rem) to indicate
+       that a zero divide check is required. 
+
+     - Do_Overflow_Check
+
+       This flag is set on an operator where an overflow check is required on
+       the operation.
+*)
+
+
+(** ** run time checks *)
+(** checks that are needed to be performed in run time *)
+Inductive run_time_checks: Type := 
+    | Do_Division_Check: run_time_checks
+    | Do_Overflow_Check: run_time_checks.
+
+Definition run_time_check_set := list run_time_checks.
+
+(** produce check flags for expressions according to the checking rules; 
+    Note: for division operator, now we only consider the division by 
+    zero check, later we will extend it by with overflow checks, and
+    it will be a mapping from one ast node to a set of run time checks;
+*)
+Inductive check_flags: expression -> run_time_check_set -> Prop :=
+    | CF_Literal_Int: forall ast_num n,
+        check_flags (E_Literal ast_num (Integer_Literal n)) nil
+    | CF_Literal_Bool: forall ast_num b,
+        check_flags (E_Literal ast_num (Boolean_Literal b)) nil
+    | CF_Identifier: forall ast_num x,  
+        check_flags (E_Identifier ast_num x) nil
+    | CF_Binary_Operation_Plus: forall ast_num e1 e2,
+        check_flags (E_Binary_Operation ast_num Plus e1 e2) (Do_Overflow_Check :: nil)
+    | CF_Binary_Operation_Minus: forall ast_num e1 e2,
+        check_flags (E_Binary_Operation ast_num Minus e1 e2) (Do_Overflow_Check :: nil)
+    | CF_Binary_Operation_Multiply: forall ast_num e1 e2,
+        check_flags (E_Binary_Operation ast_num Multiply e1 e2) (Do_Overflow_Check :: nil)
+    | CF_Binary_Operation_Div: forall ast_num e1 e2,
+        check_flags (E_Binary_Operation ast_num Divide e1 e2) (Do_Division_Check :: Do_Overflow_Check :: nil)
+    | CF_Binary_Operation_Others: forall ast_num op e1 e2,
+        op <> Plus ->
+        op <> Minus ->
+        op <> Multiply ->
+        op <> Divide ->
+        check_flags (E_Binary_Operation ast_num op e1 e2) nil
+    | CF_Unary_Operation: forall ast_num op e, (* extend  with more unary operators later *)
+        check_flags (E_Unary_Operation ast_num op e) nil.
+
+(** ** semantics for run time checks *)
+(** 32-bit integer is in the range of min_signed and max_signed, where
+    min_signed: -2^31 
+    max_signed: 2^31-1
+    
+    if v1 = -2^31 and v2 = -1 then v1/v2 = 2^31, which is out of its range; 
+*)
+Inductive do_check: binary_operator -> value -> value -> bool -> Prop :=
+    | Do_Overflow_Check_On_Plus: forall v1 v2 b,
+        (* min_signed <= (v1 + v2) <= max_signed *)
+        (Zge_bool (v1 + v2) min_signed) && (Zle_bool (v1 + v2) max_signed) = b ->
+        do_check Plus (Int v1) (Int v2) b
+    | Do_Overflow_Check_On_Minus: forall v1 v2 b,
+        (* min_signed <= (v1 - v2) <= max_signed *)
+        (Zge_bool (v1 - v2) min_signed) && (Zle_bool (v1 - v2) max_signed) = b ->
+        do_check Minus (Int v1) (Int v2) b
+    | Do_Overflow_Check_On_Multiply: forall v1 v2 b,
+        (* min_signed <= (v1 * v2) <= max_signed *)
+        (Zge_bool (v1 * v2) min_signed) && (Zle_bool (v1 * v2) max_signed) = b ->
+        do_check Multiply (Int v1) (Int v2) b
+    | Do_Division_By_Zero_And_Overflow_Check_On_Divide: forall v1 v2 b,
+        (* min_signed <= (v1 / v2) <= max_signed and v2 is not zero *)
+        (* (negb (Zeq_bool v2 0)) && (Zeq_bool v1 min_signed) && (Zeq_bool v2 (-1)) = b -> *)
+        (negb (Zeq_bool v2 0)) && ((Zge_bool (v1 / v2) min_signed) && (Zle_bool (v1 / v2) max_signed)) = b ->
+        do_check Divide (Int v1) (Int v2) b
+    | Do_Nothing: forall op v1 v2,
+        op <> Plus ->
+        op <> Minus ->
+        op <> Multiply ->
+        op <> Divide ->
+        do_check op v1 v2 true.
+
+(** do run time check only when the operator is labled with certain check flags  *)
+
+Inductive do_flagged_check: run_time_checks -> binary_operator -> value -> value -> bool -> Prop :=
+    | Do_Overflow_Check_Plus: forall v1 v2 b,
+        (Zge_bool (v1 + v2) min_signed) && (Zle_bool (v1 + v2) max_signed) = b ->
+        do_flagged_check Do_Overflow_Check Plus (Int v1) (Int v2) b
+    | Do_Overflow_Check_Minus: forall v1 v2 b,
+        (Zge_bool (v1 - v2) min_signed) && (Zle_bool (v1 - v2) max_signed) = b ->
+        do_flagged_check Do_Overflow_Check Minus (Int v1) (Int v2) b
+    | Do_Overflow_Check_Multiply: forall v1 v2 b,
+        (Zge_bool (v1 * v2) min_signed) && (Zle_bool (v1 * v2) max_signed) = b ->
+        do_flagged_check Do_Overflow_Check Multiply (Int v1) (Int v2) b
+    | Do_Overflow_Check_Divide: forall v1 v2 b,
+        (* (Zeq_bool v1 min_signed) && (Zeq_bool v2 (-1)) = b -> *)
+        (Zge_bool (v1 / v2) min_signed) && (Zle_bool (v1 / v2) max_signed) = b ->
+        do_flagged_check Do_Overflow_Check Divide (Int v1) (Int v2) b
+    | Do_Division_By_Zero_Check: forall v1 v2 b,
+        negb (Zeq_bool v2 0) = b ->
+        do_flagged_check Do_Division_Check Divide (Int v1) (Int v2) b.
+
+Inductive do_flagged_checks: run_time_check_set -> binary_operator -> value -> value -> bool -> Prop :=
+    | Do_No_Check: forall op v1 v2,
+        do_flagged_checks nil op v1 v2 true
+    | Do_Checks_False: forall ck op v1 v2 cks,
+        do_flagged_check ck op v1 v2 false ->
+        do_flagged_checks (ck :: cks) op v1 v2 false
+    | Do_Checks_True: forall ck op v1 v2 cks b,
+        do_flagged_check ck op v1 v2 true ->
+        do_flagged_checks cks op v1 v2 b ->
+        do_flagged_checks (ck :: cks) op v1 v2 b.
+
+
+(** ** Functional semantics *)
+
+(** Function for run-time checks generation according to checking rules *)
+
+Function f_check_flags (e: expression): run_time_check_set :=
+    match e with
+    | E_Literal ast_num n => nil
+    | E_Identifier ast_num x => nil
+    | E_Binary_Operation ast_num op e1 e2 => 
+        match op with
+        | Plus => (Do_Overflow_Check :: nil)
+        | Minus => (Do_Overflow_Check :: nil)
+        | Multiply => (Do_Overflow_Check :: nil)
+        | Divide => (Do_Division_Check :: Do_Overflow_Check :: nil)
+        | _ => nil
+        end
+    | E_Unary_Operation ast_num op e => nil
+    end.
+
+Function f_do_check (op: binary_operator) (v1: value) (v2: value): option bool :=
+    match op with
+    | Plus => (* overflow check *)
+        match v1, v2 with
+        | Int v1', Int v2' => Some ((Zge_bool (v1' + v2') min_signed) && (Zle_bool (v1' + v2') max_signed))
+        | _, _ => None
+        end
+    | Minus => (* overflow check *)
+        match v1, v2 with
+        | Int v1', Int v2' => Some ((Zge_bool (v1' - v2') min_signed) && (Zle_bool (v1' - v2') max_signed))
+        | _, _ => None
+        end
+    | Multiply => (* overflow check *)
+        match v1, v2 with
+        | Int v1', Int v2' => Some ((Zge_bool (v1' * v2') min_signed) && (Zle_bool (v1' * v2') max_signed))
+        | _, _ => None
+        end
+    | Divide => (* both division by zero check and overflow check *)
+        match v1, v2 with
+        | Int v1', Int v2' => 
+            Some ((negb (Zeq_bool v2' 0)) && ((Zge_bool (v1' / v2') min_signed) && (Zle_bool (v1' / v2') max_signed)))
+        | _, _ => None
+        end
+    | _ => Some true
+    end.
+
+(** only do Do_Division_Check on Divide make sense, so 
+    Do_Division_Check on other operators returns None;
+*)
+Function f_do_flagged_check (rtc: run_time_checks) (op: binary_operator) (v1: value) (v2: value): option bool :=
+    match rtc, op with
+    | Do_Overflow_Check, Plus => 
+        match v1, v2 with
+        | Int v1', Int v2' => Some ((Zge_bool (v1' + v2') min_signed) && (Zle_bool (v1' + v2') max_signed))
+        | _, _ => None
+        end
+    | Do_Overflow_Check, Minus => 
+        match v1, v2 with
+        | Int v1', Int v2' => Some ((Zge_bool (v1' - v2') min_signed) && (Zle_bool (v1' - v2') max_signed))
+        | _, _ => None
+        end
+    | Do_Overflow_Check, Multiply => 
+        match v1, v2 with
+        | Int v1', Int v2' => Some ((Zge_bool (v1' * v2') min_signed) && (Zle_bool (v1' * v2') max_signed))
+        | _, _ => None
+        end
+    | Do_Overflow_Check, Divide => 
+        match v1, v2 with
+        | Int v1', Int v2' => Some ((Zge_bool (v1' / v2') min_signed) && (Zle_bool (v1' / v2') max_signed))
+        | _, _ => None
+        end
+    | Do_Division_Check, Divide => 
+        match v1, v2 with
+        | Int v1', Int v2' => Some (negb (Zeq_bool v2' 0))
+        | _, _ => None
+        end
+    | _, _ => None
+    end.
+
+Function f_do_flagged_checks (rtcs: run_time_check_set) (op: binary_operator) (v1: value) (v2: value): option bool :=
+    match rtcs with
+    | nil => Some true
+    | rtc :: rtcs' => 
+        match f_do_flagged_check rtc op v1 v2 with
+        | Some false => Some false
+        | Some true => f_do_flagged_checks rtcs' op v1 v2
+        | None => None
+        end
+    end.
+
+
+(** ** Bisimulation between relational and functional semantics *)
+
+(** bisimulation proof between f_check_flag and check_flag: 
+    - f_check_flag_correct
+    - f_check_flag_complete
+*)
+Lemma f_check_flags_correct: forall e cks,
+    f_check_flags e = cks ->
+    check_flags e cks.
+Proof.
+    intros e;
+    functional induction (f_check_flags e);
+    intros ck h1;
+    rewrite <- h1;
+    try constructor;
+    match goal with
+    | |- ?op <> Plus => idtac
+    | |- ?op <> Minus => idtac
+    | |- ?op <> Multiply => idtac
+    | |- ?op <> Divide => idtac
+    | _ => destruct n; constructor
+    end;
+    destruct op; inversion y;
+    unfold not; intros hz1; inversion hz1.
+Qed.
+
+Lemma f_check_flags_complete: forall e cks,
+    check_flags e cks ->
+    f_check_flags e = cks.
+Proof.
+    intros e ck h1.
+    induction h1;
+    auto.
+    destruct op; intuition.
+Qed.
+
+
+(** bisimulation proof between f_do_check and do_check: 
+    - f_do_check_correct
+    - f_do_check_complete
+*)
+Lemma f_do_check_correct: forall op v1 v2 b,
+    f_do_check op v1 v2 = Some b ->
+    do_check op v1 v2 b.
+Proof.
+    intros op v1 v2;
+    functional induction (f_do_check op v1 v2);
+    intros b h1;
+    inversion h1; subst;
+    match goal with 
+    | |- do_check Plus ?v1 ?v2 ?v => idtac
+    | |- do_check Minus ?v1 ?v2 ?v => idtac
+    | |- do_check Multiply ?v1 ?v2 ?v => idtac
+    | |- do_check Divide ?v1 ?v2 ?v => idtac
+    | _ => destruct op; try inversion y;
+           constructor; unfold not; intros hz1;
+           inversion hz1
+    end; constructor; try (rewrite e1); auto.
+Qed.
+
+Lemma f_do_check_complete: forall op v1 v2 b,
+    do_check op v1 v2 b ->
+    f_do_check op v1 v2 = Some b.
+Proof.
+    intros op v1 v2 b h1.
+    induction h1; simpl;
+    try (rewrite H; auto).
+    destruct op; intuition.
+Qed.
+
+Lemma f_do_flagged_check_correct: forall ck op v1 v2 b,
+    f_do_flagged_check ck op v1 v2 = Some b ->
+    do_flagged_check ck op v1 v2 b.
+Proof.
+    intros ck op v1 v2;
+    functional induction (f_do_flagged_check ck op v1 v2);
+    intros b h1;
+    inversion h1; subst;
+    constructor; auto.
+Qed.
+
+Lemma f_do_flagged_check_complete: forall ck op v1 v2 b,
+    do_flagged_check ck op v1 v2 b ->
+    f_do_flagged_check ck op v1 v2 = Some b.
+Proof.
+    intros ck op v1 v2 b h1.
+    induction h1; simpl;
+    rewrite H; auto.
+Qed.
+
+Lemma f_do_flagged_checks_correct: forall cks op v1 v2 b,
+    f_do_flagged_checks cks op v1 v2 = Some b ->
+    do_flagged_checks cks op v1 v2 b.
+Proof.
+    intros cks op v1 v2;
+    functional induction (f_do_flagged_checks cks op v1 v2);
+    intros b h1.
+  - inversion h1; subst.
+    constructor.
+  - inversion h1; subst.
+    constructor.
+    apply f_do_flagged_check_correct; auto.
+  - specialize (IHo _ h1).
+    constructor; auto.
+    apply f_do_flagged_check_correct; auto.
+  - inversion h1.
+Qed.
+
+Lemma f_do_flagged_checks_complete: forall cks op v1 v2 b,
+    do_flagged_checks cks op v1 v2 b ->
+    f_do_flagged_checks cks op v1 v2 = Some b.
+Proof.
+    intros cks op v1 v2 b h1.
+    induction h1; simpl; auto.
+  - rewrite (f_do_flagged_check_complete _ _ _ _ _ H).
+    auto.
+  - rewrite (f_do_flagged_check_complete _ _ _ _ _ H).
+    auto.
+Qed.
+
+(** * Lemmas about run time checks *)
+
+Lemma do_complete_checks_correct: forall ast_num op e1 e2 cks v1 v2 b,
+    check_flags (E_Binary_Operation ast_num op e1 e2) cks ->
+    do_flagged_checks cks op v1 v2 b ->
+    do_check op v1 v2 b.
+Proof.
+    intros ast_num op e1 e2 cks v1 v2 b h1 h2.
+    destruct op;
+    match goal with
+    | h: check_flags (E_Binary_Operation _ Plus ?e1 ?e2) ?cks |- _ => idtac
+    | h: check_flags (E_Binary_Operation _ Minus ?e1 ?e2) ?cks |- _ => idtac
+    | h: check_flags (E_Binary_Operation _ Multiply ?e1 ?e2) ?cks |- _ => idtac
+    | h: check_flags (E_Binary_Operation _ Divide ?e1 ?e2) ?cks |- _ => idtac
+    | h: check_flags (E_Binary_Operation _ ?op ?e1 ?e2) ?cks |- _ => 
+        inversion h1; subst; inversion h2; subst; constructor; rm_always_true
+    end.
+  - (* Plus *)
+    inversion h1; subst.
+    + destruct b.
+      * inversion h2; subst.
+        inversion H1; subst.
+        constructor; auto.
+      * inversion h2; subst.
+        inversion H4; subst.
+        constructor; auto.
+        inversion H6.
+    + rm_false_hyp.
+  - (* Minus *)
+    inversion h1; subst.
+    + destruct b.
+      * inversion h2; subst.
+        inversion H1; subst.
+        constructor; auto.
+      * inversion h2; subst.
+        inversion H4; subst.
+        constructor; auto.
+        inversion H6.
+    + rm_false_hyp.
+  - (* Multiply *)
+    inversion h1; subst.
+    + destruct b.
+      * inversion h2; subst.
+        inversion H1; subst.
+        constructor; auto.
+      * inversion h2; subst.
+        inversion H4; subst.
+        constructor; auto.
+        inversion H6.
+    + rm_false_hyp.
+  - (* Divide *)
+    inversion h1; subst.
+    + destruct b.
+      * inversion h2; subst.
+        inversion H6; subst.
+        inversion H2; subst.
+        inversion H1; subst.
+        constructor; intuition.
+      * inversion h2; subst.
+        inversion H4; subst.
+        constructor; auto.
+        rewrite H; auto.
+        inversion H6; subst.
+        inversion H5; subst.
+        constructor. 
+        rewrite H. destruct (Zeq_bool v3 0); auto.
+        inversion H8.
+    + rm_false_hyp.
+Qed.
+
+
+Lemma do_complete_checks_correct': forall ast_num op e1 e2 cks v1 v2 b,
+    check_flags (E_Binary_Operation ast_num op e1 e2) cks ->
+    do_check op v1 v2 b ->
+    do_flagged_checks cks op v1 v2 b.
+Proof.
+    intros ast_num op e1 e2 cks v1 v2 b h1 h2.
+    destruct op;
+    match goal with
+    | h: check_flags (E_Binary_Operation _ Plus ?e1 ?e2) ?cks |- _ => idtac
+    | h: check_flags (E_Binary_Operation _ Minus ?e1 ?e2) ?cks |- _ => idtac
+    | h: check_flags (E_Binary_Operation _ Multiply ?e1 ?e2) ?cks |- _ => idtac
+    | h: check_flags (E_Binary_Operation _ Divide ?e1 ?e2) ?cks |- _ => idtac
+    | h: check_flags (E_Binary_Operation _ ?op ?e1 ?e2) ?cks |- _ => 
+        inversion h1; subst; inversion h2; subst; constructor
+    end.
+  - (* Plus *)
+    inversion h1; subst.
+    + destruct b.
+      * inversion h2; subst.
+        repeat constructor; auto.
+        rm_false_hyp.
+      * inversion h2; subst.
+        repeat constructor; auto.
+    + rm_false_hyp.
+  - (* Minus *)
+    inversion h1; subst.
+    + destruct b.
+      * inversion h2; subst.
+        repeat constructor; auto.
+        rm_false_hyp.
+      * inversion h2; subst.
+        repeat constructor; auto.
+    + rm_false_hyp.
+  - (* Multiply *)
+    inversion h1; subst.
+    + destruct b.
+      * inversion h2; subst.
+        repeat constructor; auto.
+        rm_false_hyp.
+      * inversion h2; subst.
+        repeat constructor; auto.
+    + rm_false_hyp.
+  - (* Divide *)
+    inversion h1; subst.
+    + destruct b.
+      * inversion h2; subst.
+        repeat constructor;
+        destruct (Zeq_bool v3 0); inversion H; auto.
+        rm_false_hyp.
+      * inversion h2; subst.
+        remember (negb (Zeq_bool v3 0)) as x.
+        symmetry in Heqx; destruct x; simpl in H.
+        apply Do_Checks_True;
+        repeat constructor; auto.
+        repeat constructor; auto.
+    + rm_false_hyp.
+Qed.
+
+
+(** 
+    this lemma is used only to prove binop_rule2, which means that
+    run time checks on a binary operator with two integer values 
+    should always return a value b, which can be either true or false;
+*)
+
+Lemma do_check_result_ex: forall op v1 v2,
+    exists b : bool, do_check op (Int v1) (Int v2) b.
+Proof.
+    intros op v1 v2.
+    destruct op;   
+    try match goal with
+    | [ |- exists r : bool, do_check Plus (Int ?v1) (Int ?v2) r ] => idtac
+    | [ |- exists r : bool, do_check Minus (Int ?v1) (Int ?v2) r ] => idtac
+    | [ |- exists r : bool, do_check Multiply (Int ?v1) (Int ?v2) r ] => idtac
+    | [ |- exists r : bool, do_check Divide (Int ?v1) (Int ?v2) r ] => idtac
+    | [ |- exists r : bool, do_check ?op (Int ?v1) (Int ?v2) r ] =>
+            exists true; constructor; rm_always_true
+    end.
+    + (* Plus *)
+      remember ((Zge_bool (v1 + v2) min_signed) && (Zle_bool (v1 + v2) max_signed)) as b.
+      destruct b;
+      [exists true | exists false];
+      constructor; auto.
+    + (* Minus *)
+      remember ((Zge_bool (v1 - v2) min_signed) && (Zle_bool (v1 - v2) max_signed)) as b.
+      destruct b;
+      [exists true | exists false];
+      constructor; auto.
+    + (* Multiply *)
+      remember ((Zge_bool (v1 * v2) min_signed) && (Zle_bool (v1 * v2) max_signed)) as b.
+      destruct b;
+      [exists true | exists false];
+      constructor; auto.
+    + (* Divide *)
+      destruct v2.
+      * exists false; 
+        constructor; auto.
+      * remember ((Zge_bool (v1 / (Z.pos p)) min_signed) && (Zle_bool (v1 / (Z.pos p)) max_signed)) as b.
+        destruct b;
+        [exists true | exists false];
+        constructor; auto.
+      * remember ((Zge_bool (v1 / (Z.neg p)) min_signed) && (Zle_bool (v1 / (Z.neg p)) max_signed)) as b.
+        destruct b;
+        [exists true | exists false];
+        constructor; auto.
+Qed.
+
